sha224sum.lean
@@ -12,4 +12,4 @@ import Crypto.SHA2
 open Crypto.CLI
 
 def main (args : List String) : IO UInt32 :=
-  runHashSumMain HashAlgorithm.sha224 args
+  runHashSumMain Crypto.Hash.Algorithm.sha224 args
